backend/Mach.v
@@ -266,7 +266,7 @@ Inductive state `{memory_model_ops: Mem.MemoryModelOps}: Type :=
       forall (stack: list stackframe)  (**r call stack *)
              (f: block)                (**r pointer to function to call *)
              (rs: regset)              (**r register state *)
-             (m: mem),                 (**r memory state *)
+             (m: mem) (tc: bool),                 (**r memory state *)
       state
   | Returnstate:
       forall (stack: list stackframe)  (**r call stack *)
@@ -356,7 +356,7 @@ Inductive step: state -> trace -> state -> Prop :=
       return_address_offset f c ra ->
       step (State s fb (Vptr sp Ptrofs.zero) (Mcall sig ros :: c) rs m)
         E0 (Callstate (Stackframe fb sp (Vptr fb ra) c :: s)
-                       f' rs m)
+                       f' rs m false)
   | exec_Mtailcall:
       forall s fb stk soff sig ros c rs m f f' m_ m',
       find_function_ptr ge ros rs = Some f' ->
@@ -364,9 +364,8 @@ Inductive step: state -> trace -> state -> Prop :=
       (* load_stack m (Vptr stk soff) Tptr f.(fn_link_ofs) = Some (parent_sp s) -> *)
       load_stack m (Vptr stk soff) Tptr f.(fn_retaddr_ofs) = Some (parent_ra s) ->
       Mem.free m stk (Ptrofs.unsigned soff) (Ptrofs.unsigned soff + f.(fn_stacksize)) = Some m_ ->
-      Mem.unrecord_stack_block m_ = Some m' ->
       step (State s fb (Vptr stk soff) (Mtailcall sig ros :: c) rs m)
-        E0 (Callstate s f' rs m')
+        E0 (Callstate s f' rs m' true)
   | exec_Mbuiltin:
       forall s f sp rs m ef args res b vargs t vres rs' m',
       eval_builtin_args ge rs sp m args vargs ->
@@ -414,16 +413,17 @@ Inductive step: state -> trace -> state -> Prop :=
       step (State s fb (Vptr stk soff) (Mreturn :: c) rs m)
         E0 (Returnstate s rs m')
   | exec_function_internal:
-      forall s fb rs m f m1 m1_ m3 stk rs',
+      forall s fb rs m f m1 m1_ m3 stk rs' (tc: bool),
         Genv.find_funct_ptr ge fb = Some (Internal f) ->
         check_alloc_frame (fn_frame f) f  ->
       Mem.alloc m 0 f.(fn_stacksize) = (m1, stk) ->
       let sp := Vptr stk Ptrofs.zero in
       (* store_stack m1 sp Tptr f.(fn_link_ofs) (parent_sp s) = Some m2 -> *)
       store_stack m1 sp Tptr f.(fn_retaddr_ofs) (parent_ra s) = Some m3 ->
-      Mem.record_stack_blocks m3 (make_singleton_frame_adt' stk (fn_frame f) (fn_stacksize f)) = Some m1_ ->
+      Mem.record_stack_blocks (if tc then m3 else Mem.push_new_stage m3)
+                              (make_singleton_frame_adt' stk (fn_frame f) (fn_stacksize f)) = Some m1_ ->
       rs' = undef_regs destroyed_at_function_entry rs ->
-      step (Callstate s fb rs m)
+      step (Callstate s fb rs m tc)
         E0 (State s fb sp f.(fn_code) rs' m1_)
   | exec_function_external:
       forall s fb rs m t rs' ef args res m',
@@ -442,7 +442,7 @@ Inductive step: state -> trace -> state -> Prop :=
       frame of the hypothetical caller.*)
       external_call ef ge args m t res m' ->
       rs' = set_pair (loc_result (ef_sig ef)) res (undef_regs destroyed_at_call rs) ->
-      step (Callstate s fb rs m)
+      step (Callstate s fb rs m false)
          t (Returnstate s rs' m')
   | exec_return:
       forall s f sp ra c rs m,
@@ -458,7 +458,7 @@ Inductive initial_state (p: program): state -> Prop :=
       Genv.find_symbol ge p.(prog_main) = Some fb ->
       Mem.alloc m0 0 0 = (m1,b) ->
       Mem.record_stack_blocks (Mem.push_new_stage m1) (make_singleton_frame_adt b 0 0) = Some m2 ->
-      initial_state p (Callstate nil fb (Regmap.init Vundef) m2).
+      initial_state p (Callstate nil fb (Regmap.init Vundef) m2 false).
 
 Inductive final_state: state -> int -> Prop :=
   | final_state_intro: forall rs m r retcode,
